coq/theories/imp2asm/ImpToASMCodegenDerivations.v
@@ -1,0 +1,459 @@
+From impboot Require Import utils.Core.
+Require Import impboot.assembly.ASMSyntax.
+Require Import impboot.imperative.ImpSyntax.
+Require Import impboot.utils.AppList.
+Require Import impboot.imp2asm.ImpToASMCodegen.
+From impboot Require Import automation.Ltac2Utils.
+From impboot Require Import functional.FunValues.
+From impboot Require Import functional.FunSemantics.
+Require Import impboot.automation.AutomationHOLStyle.
+Require Import coqutil.Word.Interface.
+Require Import ZArith.
+From Coq Require Import FunInd.
+From Coq Require Import derive.Derive.
+From Coq Require Import Lia.
+From Ltac2 Require Import Ltac2.
+
+Open Scope app_list_scope.
+
+(* *********************************************** *)
+(*       Derivations for Codegen Functions         *)
+(* *********************************************** *)
+
+(* Equation lemmas for Function declarations *)
+
+(* Lemma c_exp_equation : ltac:(unfold_tpe c_exp).
+Proof. ltac1:(unfold_proof). Qed.
+
+Lemma c_exps_equation : ltac:(unfold_tpe c_exps).
+Proof. ltac1:(unfold_proof). Qed.
+
+Lemma c_test_jump_equation : ltac:(unfold_tpe c_test_jump).
+Proof. ltac1:(unfold_proof). Qed.
+
+Lemma lookup_equation : ltac:(unfold_tpe lookup).
+Proof. ltac1:(unfold_proof). Qed.
+
+Lemma call_v_stack_equation : ltac:(unfold_tpe call_v_stack).
+Proof. ltac1:(unfold_proof). Qed.
+
+Lemma c_cmd_equation : ltac:(unfold_tpe c_cmd).
+Proof. ltac1:(unfold_proof). Qed.
+
+Lemma make_vs_from_binders_equation : ltac:(unfold_tpe make_vs_from_binders).
+Proof. ltac1:(unfold_proof). Qed.
+
+Lemma c_fundefs_equation : ltac:(unfold_tpe c_fundefs).
+Proof. ltac1:(unfold_proof). Qed. *)
+
+(* Equation lemmas for Fixpoint declarations *)
+
+(* Lemma c_declare_binders_rec_equation : ltac:(unfold_tpe c_declare_binders_rec).
+Proof. ltac1:(unfold_proof). Qed.
+
+Lemma all_binders_equation : ltac:(unfold_tpe all_binders).
+Proof. ltac1:(unfold_proof). Qed.
+
+Lemma names_contain_equation : ltac:(unfold_tpe names_contain).
+Proof. ltac1:(unfold_proof). Qed.
+
+Lemma names_unique_equation : ltac:(unfold_tpe names_unique).
+Proof. ltac1:(unfold_proof). Qed. *)
+
+(* Derivations for simple definitions (no dependencies) *)
+
+Opaque encode.
+Opaque name_enc.
+
+Derive init_prog 
+  in ltac2:(relcompile_tpe 'init_prog 'init []) 
+  as init_prog_proof.
+Proof.
+  intros.
+  subst init_prog.
+  relcompile.
+  all: try ltac1:(lia).
+  2: eapply FEnv.lookup_insert_eq.
+  ltac1:(replace (N.of_nat (2 ^ 63 - 1)) with (2 ^ 63 - 1)%N).
+  1: ltac1:(lia).
+  rewrite Nnat.Nat2N.inj_sub.
+  rewrite Nnat.Nat2N.inj_pow.
+  ltac1:(lia).
+Qed.
+
+Derive give_up_prog 
+  in ltac2:(relcompile_tpe 'give_up_prog 'give_up []) 
+  as give_up_prog_proof.
+Proof.
+  intros.
+  subst give_up_prog.
+  relcompile.
+  cbn; try ltac1:(congruence); try reflexivity.
+Qed.
+
+Derive abort_prog 
+  in ltac2:(relcompile_tpe 'abort_prog 'abort []) 
+  as abort_prog_proof.
+Proof.
+  intros.
+  subst abort_prog.
+  relcompile.
+  cbn; try ltac1:(congruence); try reflexivity.
+Qed.
+
+Derive c_const_prog
+  in ltac2:(relcompile_tpe 'c_const_prog 'c_const []) 
+  as c_const_prog_proof.
+Proof.
+  intros.
+  subst c_const_prog.
+  relcompile.
+  all: simpl.
+  all: cbn; try ltac1:(congruence); try reflexivity.
+Qed.
+
+(* Derivations with dependencies *)
+
+Derive even_len_prog 
+  in ltac2:(relcompile_tpe 'even_len_prog 'even_len []) 
+  as even_len_prog_proof.
+Proof.
+  intros.
+  subst even_len_prog.
+  relcompile.
+  all: inversion H0.
+Qed.
+
+Derive odd_len_prog 
+  in ltac2:(relcompile_tpe 'odd_len_prog 'odd_len []) 
+  as odd_len_prog_proof.
+Proof.
+  intros.
+  subst odd_len_prog.
+  relcompile.
+  all: inversion H0.
+Qed.
+
+Derive index_of_prog 
+  in ltac2:(relcompile_tpe 'index_of_prog 'index_of ['index_of]) 
+  as index_of_prog_proof.
+Proof.
+  intros.
+  subst index_of_prog.
+  relcompile.
+  all: simpl; eauto.
+  all: cbn; try ltac1:(congruence); try reflexivity.
+  1: exact Refinable_nat.
+  1: inversion H1.
+  all: cbn; try ltac1:(congruence); try reflexivity.
+Qed.
+
+Derive index_of_opt_prog 
+  in ltac2:(relcompile_tpe 'index_of_opt_prog 'index_of_opt []) 
+  as index_of_opt_prog_proof.
+Proof.
+  intros.
+  subst index_of_opt_prog.
+  relcompile.
+Qed.
+
+Derive c_var_prog 
+  in ltac2:(relcompile_tpe 'c_var_prog 'c_var ['index_of]) 
+  as c_var_prog_proof.
+Proof.
+  intros.
+  subst c_var_prog.
+  relcompile.
+Qed.
+
+Derive c_declare_binders_rec_prog 
+  in ltac2:(relcompile_tpe 'c_declare_binders_rec_prog 'c_declare_binders_rec []) 
+  as c_declare_binders_rec_prog_proof.
+Proof.
+  intros.
+  subst c_declare_binders_rec_prog.
+  relcompile.
+Qed.
+
+Derive c_declare_binders_prog 
+  in ltac2:(relcompile_tpe 'c_declare_binders_prog 'c_declare_binders ['c_declare_binders_rec]) 
+  as c_declare_binders_prog_proof.
+Proof.
+  intros.
+  subst c_declare_binders_prog.
+  relcompile.
+Qed.
+
+Derive c_assign_prog 
+  in ltac2:(relcompile_tpe 'c_assign_prog 'c_assign ['index_of]) 
+  as c_assign_prog_proof.
+Proof.
+  intros.
+  subst c_assign_prog.
+  relcompile.
+Qed.
+
+Derive c_add_prog 
+  in ltac2:(relcompile_tpe 'c_add_prog 'c_add []) 
+  as c_add_prog_proof.
+Proof.
+  intros.
+  subst c_add_prog.
+  relcompile.
+Qed.
+
+Derive c_sub_prog 
+  in ltac2:(relcompile_tpe 'c_sub_prog 'c_sub []) 
+  as c_sub_prog_proof.
+Proof.
+  intros.
+  subst c_sub_prog.
+  relcompile.
+Qed.
+
+Derive c_div_prog 
+  in ltac2:(relcompile_tpe 'c_div_prog 'c_div []) 
+  as c_div_prog_proof.
+Proof.
+  intros.
+  subst c_div_prog.
+  relcompile.
+Qed.
+
+Derive c_alloc_prog 
+  in ltac2:(relcompile_tpe 'c_alloc_prog 'c_alloc ['even_len]) 
+  as c_alloc_prog_proof.
+Proof.
+  intros.
+  subst c_alloc_prog.
+  relcompile.
+Qed.
+
+Derive align_prog 
+  in ltac2:(relcompile_tpe 'align_prog 'align []) 
+  as align_prog_proof.
+Proof.
+  intros.
+  subst align_prog.
+  relcompile.
+Qed.
+
+Derive c_read_prog 
+  in ltac2:(relcompile_tpe 'c_read_prog 'c_read ['even_len; 'align]) 
+  as c_read_prog_proof.
+Proof.
+  intros.
+  subst c_read_prog.
+  relcompile.
+Qed.
+
+Derive c_write_prog 
+  in ltac2:(relcompile_tpe 'c_write_prog 'c_write ['even_len; 'align]) 
+  as c_write_prog_proof.
+Proof.
+  intros.
+  subst c_write_prog.
+  relcompile.
+Qed.
+
+Derive c_load_prog 
+  in ltac2:(relcompile_tpe 'c_load_prog 'c_load []) 
+  as c_load_prog_proof.
+Proof.
+  intros.
+  subst c_load_prog.
+  relcompile.
+Qed.
+
+Derive c_store_prog 
+  in ltac2:(relcompile_tpe 'c_store_prog 'c_store []) 
+  as c_store_prog_proof.
+Proof.
+  intros.
+  subst c_store_prog.
+  relcompile.
+Qed.
+
+Derive c_exp_prog 
+  in ltac2:(relcompile_tpe 'c_exp_prog 'c_exp ['c_var; 'c_const; 'c_add; 'c_sub; 'c_div; 'c_load]) 
+  as c_exp_prog_proof.
+Proof.
+  intros.
+  subst c_exp_prog.
+  relcompile.
+Qed.
+
+Derive c_exps_prog 
+  in ltac2:(relcompile_tpe 'c_exps_prog 'c_exps ['c_exp]) 
+  as c_exps_prog_proof.
+Proof.
+  intros.
+  subst c_exps_prog.
+  relcompile.
+Qed.
+
+Derive c_cmp_prog 
+  in ltac2:(relcompile_tpe 'c_cmp_prog 'c_cmp []) 
+  as c_cmp_prog_proof.
+Proof.
+  intros.
+  subst c_cmp_prog.
+  relcompile.
+Qed.
+
+Derive c_test_jump_prog 
+  in ltac2:(relcompile_tpe 'c_test_jump_prog 'c_test_jump ['c_exp; 'c_cmp]) 
+  as c_test_jump_prog_proof.
+Proof.
+  intros.
+  subst c_test_jump_prog.
+  relcompile.
+Qed.
+
+Derive lookup_prog 
+  in ltac2:(relcompile_tpe 'lookup_prog 'lookup []) 
+  as lookup_prog_proof.
+Proof.
+  intros.
+  subst lookup_prog.
+  relcompile.
+Qed.
+
+Derive make_ret_prog 
+  in ltac2:(relcompile_tpe 'make_ret_prog 'make_ret []) 
+  as make_ret_prog_proof.
+Proof.
+  intros.
+  subst make_ret_prog.
+  relcompile.
+Qed.
+
+Derive c_pops_prog 
+  in ltac2:(relcompile_tpe 'c_pops_prog 'c_pops ['give_up; 'even_len]) 
+  as c_pops_prog_proof.
+Proof.
+  intros.
+  subst c_pops_prog.
+  relcompile.
+Qed.
+
+Derive call_v_stack_prog 
+  in ltac2:(relcompile_tpe 'call_v_stack_prog 'call_v_stack []) 
+  as call_v_stack_prog_proof.
+Proof.
+  intros.
+  subst call_v_stack_prog.
+  relcompile.
+Qed.
+
+Derive c_pushes_prog 
+  in ltac2:(relcompile_tpe 'c_pushes_prog 'c_pushes ['call_v_stack]) 
+  as c_pushes_prog_proof.
+Proof.
+  intros.
+  subst c_pushes_prog.
+  relcompile.
+Qed.
+
+Derive c_call_prog 
+  in ltac2:(relcompile_tpe 'c_call_prog 'c_call ['c_pops; 'align; 'even_len]) 
+  as c_call_prog_proof.
+Proof.
+  intros.
+  subst c_call_prog.
+  relcompile.
+Qed.
+
+Derive c_cmd_prog 
+  in ltac2:(relcompile_tpe 'c_cmd_prog 'c_cmd 
+    ['c_exp; 'c_assign; 'c_store; 'c_test_jump; 'c_exps; 'c_call; 
+     'c_var; 'make_ret; 'c_alloc; 'c_read; 'c_write; 'abort; 'lookup]) 
+  as c_cmd_prog_proof.
+Proof.
+  intros.
+  subst c_cmd_prog.
+  relcompile.
+Qed.
+
+Derive all_binders_prog 
+  in ltac2:(relcompile_tpe 'all_binders_prog 'all_binders []) 
+  as all_binders_prog_proof.
+Proof.
+  intros.
+  subst all_binders_prog.
+  relcompile.
+Qed.
+
+Derive names_contain_prog 
+  in ltac2:(relcompile_tpe 'names_contain_prog 'names_contain []) 
+  as names_contain_prog_proof.
+Proof.
+  intros.
+  subst names_contain_prog.
+  relcompile.
+Qed.
+
+Derive names_unique_prog 
+  in ltac2:(relcompile_tpe 'names_unique_prog 'names_unique ['names_contain]) 
+  as names_unique_prog_proof.
+Proof.
+  intros.
+  subst names_unique_prog.
+  relcompile.
+Qed.
+
+Derive unique_binders_prog 
+  in ltac2:(relcompile_tpe 'unique_binders_prog 'unique_binders ['all_binders; 'names_unique]) 
+  as unique_binders_prog_proof.
+Proof.
+  intros.
+  subst unique_binders_prog.
+  relcompile.
+Qed.
+
+Derive make_vs_from_binders_prog 
+  in ltac2:(relcompile_tpe 'make_vs_from_binders_prog 'make_vs_from_binders []) 
+  as make_vs_from_binders_prog_proof.
+Proof.
+  intros.
+  subst make_vs_from_binders_prog.
+  relcompile.
+Qed.
+
+Derive c_fundef_prog 
+  in ltac2:(relcompile_tpe 'c_fundef_prog 'c_fundef 
+    ['c_pushes; 'unique_binders; 'make_vs_from_binders; 'c_cmd]) 
+  as c_fundef_prog_proof.
+Proof.
+  intros.
+  subst c_fundef_prog.
+  relcompile.
+Qed.
+
+Derive name2str_prog 
+  in ltac2:(relcompile_tpe 'name2str_prog 'name2str []) 
+  as name2str_prog_proof.
+Proof.
+  intros.
+  subst name2str_prog.
+  relcompile.
+Qed.
+
+Derive c_fundefs_prog 
+  in ltac2:(relcompile_tpe 'c_fundefs_prog 'c_fundefs ['c_fundef; 'name2str]) 
+  as c_fundefs_prog_proof.
+Proof.
+  intros.
+  subst c_fundefs_prog.
+  relcompile.
+Qed.
+
+Derive codegen_prog 
+  in ltac2:(relcompile_tpe 'codegen_prog 'codegen ['c_fundefs; 'lookup; 'init]) 
+  as codegen_prog_proof.
+Proof.
+  intros.
+  subst codegen_prog.
+  relcompile.
+Qed.
+
